wip

proof/correctness/Repr2.ec
@@ -1,6 +1,6 @@
 pragma Goals : printall.
 
-require import AllCore List.
+require import AllCore List IntDiv.
 
 from Jasmin require import JModel.
 
@@ -10,6 +10,7 @@ require import BitEncoding.
 (*---*) import BitChunking.
 
 require import Params WOTS.
+require import Utils2.
 
 require import Array2144.
 
@@ -39,6 +40,107 @@ op DecodeWotsPk (pk : wots_pk) : W8.t Array2144.t =
 
 op EncodeWotsSignature (s : W8.t Array2144.t) : wots_signature = 
   LenNBytes.insubd (map NBytes.insubd (chunk 32 (to_list s))). 
+
+op EncodeWotsPk (pk : W8.t Array2144.t) : wots_pk = 
+  LenNBytes.insubd (map NBytes.insubd (chunk 32 (to_list pk))). 
+
+(** -------------------------------------------------------------------------------------------- **)
+
+(* aux *)
+lemma enc_dec_wots_pk_r (x : W8.t Array2144.t) (y : wots_pk) :
+    len = 67 /\ n = 32 =>
+    y = EncodeWotsPk x => x = DecodeWotsPk y.
+proof.
+move => [#] len_val n_val H.
+rewrite /DecodeWotsPk H /EncodeWotsPk.
+rewrite tP => i?.
+rewrite get_of_list; 1:assumption.
+rewrite /nbytes_flatten (nth_flatten witness 32).
+  + pose P := (fun (s : W8.t list) => size s = 32).
+    pose L := (map NBytes.val (val (insubd (map NBytes.insubd (chunk 32 (to_list x)))))).
+    rewrite -(all_nthP P L witness) /L /P size_map valP.
+    rewrite insubdK; [ rewrite /P size_map size_chunk // size_to_list len_val //= |] => j?.  
+    by rewrite (nth_map witness) 1:#smt:(size_map size_chunk size_to_list) valP n_val.         
+rewrite (nth_map witness).
+  + rewrite valP /#.
+rewrite insubdK.
+  + rewrite /P size_map size_chunk // size_to_list len_val //=.
+rewrite (nth_map witness).
+  + rewrite size_chunk // size_to_list /#. 
+rewrite insubdK. 
+  + rewrite /P /chunk nth_mkseq; [rewrite size_to_list /# |] => />. 
+    rewrite size_take //= size_drop 1:/# size_to_list /#. 
+rewrite /chunk nth_mkseq 1:#smt:(size_to_list) => />.
+rewrite nth_take // 1:/# nth_drop 1,2:/# get_to_list /#. 
+qed.
+
+(* aux *)
+lemma enc_dec_wots_pk_l (x : W8.t Array2144.t) (y : wots_pk) :
+    len = 67 /\ n = 32 =>
+    x = DecodeWotsPk y => y = EncodeWotsPk x.
+proof.
+move => [#] len_val n_val H. 
+rewrite /EncodeWotsPk H /DecodeWotsPk.  
+rewrite -len_nbytes_eq. 
+apply (eq_from_nth witness).
+  + rewrite valP insubdK; [rewrite /P size_map size_chunk // size_to_list len_val //= |].  
+    rewrite size_map size_chunk // size_to_list len_val //=. 
+rewrite valP len_val => j?. 
+rewrite insubdK. 
+  + rewrite /P size_map size_chunk // size_to_list len_val //=.
+rewrite (nth_map witness). 
+  + rewrite size_chunk // size_to_list /#.
+rewrite /chunk nth_mkseq; [rewrite size_to_list //= |] => />. 
+rewrite -nbytes_eq insubdK. 
+  + rewrite /P size_take // size_drop 1:/# size_to_list n_val /#. 
+apply (eq_from_nth witness).
+  + rewrite valP size_take // size_drop 1:/# size_to_list n_val /#.
+rewrite valP n_val => i?. 
+rewrite nth_take // 1:/# nth_drop 1,2:/# get_to_list. 
+rewrite get_of_list 1:/# /nbytes_flatten (nth_flatten witness 32). 
+  + pose P := (fun (s : W8.t list) => size s = 32).
+    pose L := (map NBytes.val (val y)).
+    rewrite -(all_nthP P L witness) /L /P size_map valP len_val => ??.
+    rewrite (nth_map witness); [by rewrite valP len_val |].
+    rewrite valP n_val //. 
+rewrite (nth_map witness) => [| /#].
+rewrite valP len_val /#. 
+qed.
+
+lemma enc_dec_wots_pk (x : W8.t Array2144.t) (y : wots_pk) :
+    len = 67 /\ n = 32 =>
+    x = DecodeWotsPk y <=> y = EncodeWotsPk x.
+proof.
+move => [#] ??. 
+split; [apply enc_dec_wots_pk_l | apply enc_dec_wots_pk_r] => /#.
+qed.
+
+
+lemma enc_comp_dec_pk (x : W8.t Array2144.t) :
+    len = 67 /\ n = 32 =>
+    x = DecodeWotsPk (EncodeWotsPk x).
+proof.
+move => [#] len_val n_val.
+rewrite /DecodeWotsPk /EncodeWotsPk. 
+rewrite tP => j?. 
+rewrite get_of_list // insubdK. 
+  + rewrite /P size_map size_chunk // size_to_list len_val //=.
+rewrite /nbytes_flatten (nth_flatten witness 32). 
+  + pose P := (fun (s : W8.t list) => size s = 32).
+    pose L := (map NBytes.val (map NBytes.insubd (chunk 32 (to_list x)))).
+    rewrite -(all_nthP P L witness) /L /P !size_map !size_iota (: max 0 (max 0 2144 %/ 32) = 67) 1:/# => i?.  
+    rewrite (nth_map witness); [rewrite size_map size_chunk // size_to_list //= |].
+    by rewrite valP n_val. 
+rewrite (nth_map witness).
+  + rewrite size_map size_chunk // size_to_list //= /#.
+rewrite (nth_map witness).
+  + rewrite size_chunk // size_to_list //= /#.
+rewrite insubdK.
+  + rewrite /P /chunk nth_mkseq 1:#smt:(size_to_list) => />.
+    rewrite size_take // size_drop 1:/# size_to_list n_val /#. 
+rewrite /chunk nth_mkseq 1:#smt:(size_to_list) => />.
+rewrite nth_take // 1:/# nth_drop 1,2:/# get_to_list /#.
+qed.
 
 (** -------------------------------------------------------------------------------------------- **)
 
